Steel framing: Make change_sq more robust

pulse/ulib/experimental/Steel.Memory.fsti
@@ -86,8 +86,11 @@ val interp (p:slprop u#a) (m:mem u#a) : prop
 let hmem (p:slprop u#a) = m:mem u#a {interp p m}
 
 (** Equivalence relation on slprops is just equivalence of their interpretations *)
-let equiv (p1 p2:slprop) : prop =
-  forall m. interp p1 m <==> interp p2 m
+val equiv (p1 p2:slprop u#a) : prop
+
+val reveal_equiv (p1 p2:slprop u#a) : Lemma
+  (ensures (forall m. interp p1 m <==> interp p2 m) <==> p1 `equiv` p2)
+  [SMTPat (p1 `equiv` p2)]
 
 (** Implication of slprops *)
 let slimp (p1 p2 : slprop) : prop =
